Implement SatLib as a z3 network service

satNative.cs
@@ -1,0 +1,167 @@
+
+using System;
+using System.Net;
+using System.Net.Sockets;
+using System.Text;
+using System.Numerics;
+
+namespace @NetworkSatLib {
+
+  public class BoolExpr
+  {
+    public string expr;
+    public BoolExpr(string s) {
+      expr = s;
+    }
+  }
+
+  public class IntExpr
+  {
+    public string expr;
+    public IntExpr(string s) {
+      expr = s;
+    }
+  }
+
+  public partial class __default {
+
+    public static void getTrueBool(out BoolExpr e) {
+      e = new BoolExpr("True");
+    }
+    public static BoolExpr getTrueBool() {
+      BoolExpr e;
+      getTrueBool(out e);
+      return e;
+    }
+
+    public static void and(BoolExpr f1, BoolExpr f2, out BoolExpr e) {
+      e = new BoolExpr(String.Format(
+        "z3.And({0}, {1})",
+        f1.expr, f2.expr
+      ));
+    }
+    public static BoolExpr and(BoolExpr f1, BoolExpr f2) {
+      BoolExpr e;
+      and(f1, f2, out e);
+      return e;
+    }
+
+    public static void not(BoolExpr f1, out BoolExpr e) {
+      e = new BoolExpr(String.Format(
+        "z3.Not({0})",
+        f1.expr
+      ));
+    }
+    public static BoolExpr not(BoolExpr f1) {
+      BoolExpr e;
+      not(f1, out e);
+      return e;
+    }
+
+    public static void boolToInt(BoolExpr b, out IntExpr e) {
+      e = new IntExpr(String.Format(
+        "z3.If({0}, 1, 0)",
+        b.expr
+      ));
+    }
+    public static IntExpr boolToInt(BoolExpr b) {
+      IntExpr e;
+      boolToInt(b, out e);
+      return e;
+    }
+
+    public static void boolExprToStr(BoolExpr b, out string e) {
+      e = b.expr;
+    }
+    public static string boolExprToStr(BoolExpr b) {
+      string e;
+      boolExprToStr(b, out e);
+      return e;
+    }
+
+
+    public static void intConst(BigInteger i, out IntExpr e) {
+      e = new IntExpr(String.Format(
+        "z3.IntVal(\"{0}\")",
+        i
+      ));
+    }
+    public static IntExpr intConst(BigInteger i) {
+      IntExpr e;
+      intConst(i, out e);
+      return e;
+    }
+
+    public static void intSymbolic(BigInteger i, out IntExpr e) {
+      e = new IntExpr(String.Format(
+        "z3.Int(\"reg{0}\")",
+        i
+      ));
+    }
+    public static IntExpr intSymbolic(BigInteger i) {
+      IntExpr e;
+      intSymbolic(i, out e);
+      return e;
+    }
+
+    public static void add(IntExpr f1, IntExpr f2, out IntExpr e) {
+      e = new IntExpr(String.Format(
+        "({0} + {1})",
+        f1.expr, f2.expr
+      ));
+    }
+    public static IntExpr add(IntExpr f1, IntExpr f2) {
+      IntExpr e;
+      add(f1, f2, out e);
+      return e;
+    }
+
+    public static void cmp(IntExpr f1, IntExpr f2, out BoolExpr e) {
+      e = new BoolExpr(String.Format(
+        "({0} == {1})",
+        f1.expr, f2.expr
+      ));
+    }
+    public static BoolExpr cmp(IntExpr f1, IntExpr f2) {
+      BoolExpr e;
+      cmp(f1, f2, out e);
+      return e;
+    }
+
+    public static bool sat(BoolExpr f1) {
+      string answer = makeTcpRequest(f1.expr);
+      return answer == "Y";
+    }
+    public static string makeTcpRequest(string s) {
+      // Modified from: 
+      //   https://www.devarticles.com/c/a/C-Sharp/Network-Programming-in-C-sharp/1/
+      IPAddress addr = IPAddress.Loopback;
+      EndPoint ep = new IPEndPoint(addr, 8000);
+
+      Socket sock = new Socket(AddressFamily.InterNetwork,SocketType.Stream,ProtocolType.Tcp);
+      sock.Connect(ep);
+
+      string request_string = s + '\n';
+      Encoding ASCII = Encoding.ASCII;
+      Byte[] ByteGet = ASCII.GetBytes(request_string);
+      Byte[] RecvBytes = new Byte[256];
+
+      sock.Send(ByteGet, ByteGet.Length, 0);
+      Int32 bytes = sock.Receive(RecvBytes, RecvBytes.Length, 0);
+      String strRetPage = null;
+      strRetPage = strRetPage + ASCII.GetString(RecvBytes, 0, bytes);
+      while (bytes > 0)
+      {
+        bytes = sock.Receive(RecvBytes, RecvBytes.Length, 0);
+        strRetPage = strRetPage + ASCII.GetString(RecvBytes, 0, bytes);
+        //Console.WriteLine(strRetPage );
+      }
+      sock.Shutdown(SocketShutdown.Both);
+      sock.Close();
+      Console.WriteLine(strRetPage);
+      return strRetPage;
+    }
+
+  }
+
+}
