z3server.py
@@ -1,0 +1,54 @@
+
+import socket
+import sys
+
+import z3
+
+
+
+HOST = '127.0.0.1'
+PORT = 8000
+
+s = socket.socket(socket.AF_INET, socket.SOCK_STREAM)
+
+#Bind socket to local host and port
+try:
+    s.bind((HOST, PORT))
+except socket.error as msg:
+    print('Bind failed. Error Code : ' + str(msg[0]) + ' Message ' + msg[1])
+    sys.exit()
+    
+print('Socket bind complete')
+
+#Start listening on socket
+try:
+  s.listen(10)
+  print('Socket now listening')
+
+#now keep talking with the client
+  while 1:
+      #wait to accept a connection - blocking call
+      conn, addr = s.accept()
+      print('Connected with ' + addr[0] + ':' + str(addr[1]))
+      sat_string = conn.recv(4096)
+      print(sat_string)
+
+      solver = z3.Solver()
+      solver.add(eval(sat_string))
+      result = solver.check().r
+      if result == 1:
+        conn.send("Y")
+        print("Y")
+      else:
+        conn.send("N")
+        print("N")
+
+      conn.close()
+      conn = None
+      
+finally:
+  try:
+    if conn:
+      conn.close()
+  finally:
+    s.close()
