sat.dfy
@@ -1,0 +1,74 @@
+
+//TODO: Add "abstract" here once a concrete one is implemented.
+abstract module AbstractSatLib {
+
+    type BoolExpr
+    function method getTrueBool(): BoolExpr
+    function method and(f1: BoolExpr, f2: BoolExpr): BoolExpr
+    function method not(f1: BoolExpr): BoolExpr
+    function method boolToInt(b: BoolExpr): IntExpr
+    function method boolExprToStr(b: BoolExpr): string
+
+    type IntExpr
+    function method intConst(i: int): IntExpr
+    function method intSymbolic(i: int): IntExpr
+    function method add(f1: IntExpr, f2: IntExpr): IntExpr
+    function method cmp(f1: IntExpr, f2: IntExpr): BoolExpr
+
+    function method {:verify false} sat(f1: BoolExpr): bool
+
+      // Used for King Property 1
+      //TODO: Possibly derive this from simpler rules
+      ensures sat(getTrueBool())
+      ensures forall a,b :: sat(a) ==>
+        sat(and(a,b)) || sat(and(a,not(b)))
+
+      // Used for King Property 2
+      //ensures forall a :: !sat(and(a, not(a)))
+      //ensures forall a,b,c,d ::
+      //  sat(and( and(a, b), and(c, d) )) ==
+      //  sat(and( and(a, c), and(b, d) ))
+      //ensures forall a,b ::
+      //  !sat(a) ==> !sat( and(a, b) )
+      //ensures forall a,b ::
+      //  sat( and(a, b) ) ==
+      //  sat( and(b, a) )
+
+}
+
+
+extern "NetworkSatLib" module NetworkSatLib {
+
+    type {:compile false} BoolExpr
+    extern function method getTrueBool(): BoolExpr
+    extern function method and(f1: BoolExpr, f2: BoolExpr): BoolExpr
+    extern function method not(f1: BoolExpr): BoolExpr
+    extern function method boolToInt(b: BoolExpr): IntExpr
+    extern function method boolExprToStr(b: BoolExpr): string
+
+    type {:compile false} IntExpr
+    extern function method intConst(i: int): IntExpr
+    extern function method intSymbolic(i: int): IntExpr
+    extern function method add(f1: IntExpr, f2: IntExpr): IntExpr
+    extern function method cmp(f1: IntExpr, f2: IntExpr): BoolExpr
+
+    extern function method {:verify false} sat(f1: BoolExpr): bool
+
+      // Used for King Property 1
+      //TODO: Possibly derive this from simpler rules
+      ensures sat(getTrueBool())
+      ensures forall a,b :: sat(a) ==>
+        sat(and(a,b)) || sat(and(a,not(b)))
+
+      // Used for King Property 2
+      //ensures forall a :: !sat(and(a, not(a)))
+      //ensures forall a,b,c,d ::
+      //  sat(and( and(a, b), and(c, d) )) ==
+      //  sat(and( and(a, c), and(b, d) ))
+      //ensures forall a,b ::
+      //  !sat(a) ==> !sat( and(a, b) )
+      //ensures forall a,b ::
+      //  sat( and(a, b) ) ==
+      //  sat( and(b, a) )
+
+}
